Prove last assume

code/ecdsap256sha2/Hacl.Spec.ECDSA.fst
@@ -1,6 +1,6 @@
 module Hacl.Spec.ECDSA
 
-open FStar.Mul 
+open FStar.Mul
 open Hacl.Spec.ECDSAP256.Definition
 open Hacl.Spec.P256.Lemmas
 
@@ -9,18 +9,17 @@ open Lib.IntTypes
 open Lib.Sequence
 
 open Spec.Hash
-open Hacl.Spec.P256 
-
+open Hacl.Spec.P256
 open Hacl.Spec.P256.Lemmas
 
-module H = Spec.Agile.Hash
 module Def = Spec.Hash.Definitions
 
-open FStar.Math.Lemmas 
-open FStar.Math.Lib 
-
+open FStar.Math.Lemmas
+open FStar.Math.Lib
 
 (*
+// Sage scratchpad
+
 def toB(x):
     for i in range(4):
         print(((x >> i * 64) % (2 ** 64)))
@@ -51,11 +50,7 @@ print(x1 == R)
 print(Integer(x1) % primeOrder)
 print(Integer(R) % primeOrder)
 
-
-
-*)
-
-(*
+#############
 
 z = 1330795747694424120 + 14316922599628991228 * 2**64 + 308854472678183009 * 2**128 + 16765196972424757399 * 2 **192
 z = 0x44acf6b7e36c1342c2c5897204fe09504e1e2efb1a900377dbc4e7a6a133ec56
@@ -67,8 +62,6 @@ order = 115792089210356248762697446949407573529996955224135760342422259061068512
 km = inverse_mod(k, order)
 s = (km * (z + r * d)) % order
 s_ = 0x8bf77819ca05a6b2786c76262bf7371cef97b218e96f175a3ccdda2acc058903
-
-
 
 print(hex(s))
 print(s_)
@@ -92,66 +85,51 @@ u1g = basePoint * u1
 u2Q = pk * u2
 x1 = (u1g + u2Q).xy()[0]
 print(int(x1) % primeOrder == r)
+*)
 
- *)
+#set-options "--fuel 0 --ifuel 0 --z3rlimit 100"
 
-let prime = prime_p256_order 
-let nat_prime = (n: nat {n < prime})
+let prime = prime_p256_order
 
-#reset-options "--z3refresh --z3rlimit  200"
-
-val lemma_u8_less: a: uint8 -> Lemma (uint_v a < pow2 8)
-
-let lemma_u8_less a = ()
+let nat_prime = n:nat{n < prime}
 
 
-val lemma_scalar_ith: sc: lbytes 32 -> k: nat { k < 32} -> Lemma (
-  uint_v sc.[k] == nat_from_intseq_le sc / pow2 (8 * k) % pow2 8)
+val lemma_scalar_ith: sc:lbytes 32 -> k:nat{k < 32} -> Lemma
+  (v sc.[k] == nat_from_intseq_le sc / pow2 (8 * k) % pow2 8)
 
-let lemma_scalar_ith sc k = 
-  nat_from_intseq_le_slice_lemma sc k;
-  let slSc = slice sc k 32 in 
-    nat_from_intseq_le_slice_lemma slSc 1;
-    nat_from_intseq_le_lemma0  (slice slSc 0 1);
-    assert(nat_from_bytes_le slSc == uint_v sc.[k] + pow2 8 * nat_from_bytes_le (slice slSc 1 (32 - k)));
-    assert(nat_from_bytes_le sc == nat_from_intseq_le (slice sc 0 k) + pow2 (8 * k) * uint_v sc.[k] + pow2 (8 * k) * pow2 8 * nat_from_bytes_le (slice sc (k + 1) 32));
-    
-    assert(nat_from_bytes_le sc / pow2 (8 * k) % pow2 8 == (nat_from_intseq_le (slice sc 0 k) + 
-    pow2 (8 * k) * (uint_v sc.[k] + pow2 8 * nat_from_bytes_le (slice sc (k + 1) 32))) / pow2 (8 * k) % pow2 8);
-    lemma_div_plus (nat_from_intseq_le (slice sc 0 k)) (uint_v sc.[k] + pow2 8 * nat_from_bytes_le (slice sc (k + 1) 32)) (pow2 (8 * k));
-    assert( (nat_from_intseq_le (slice sc 0 k) + 
-    pow2 (8 * k) * (uint_v sc.[k] + pow2 8 * nat_from_bytes_le (slice sc (k + 1) 32))) / pow2 (8 * k) == 
-    nat_from_intseq_le (slice sc 0 k) / pow2 (8 * k) + (uint_v sc.[k] + pow2 8 * nat_from_bytes_le (slice sc (k + 1) 32)));
-    
-    assert(nat_from_bytes_le sc / pow2 (8 * k) % pow2 8 ==  (nat_from_intseq_le (slice sc 0 k) / pow2 (8 * k) + (uint_v sc.[k] + pow2 8 * nat_from_bytes_le (slice sc (k + 1) 32))) % pow2 8);
+let lemma_scalar_ith sc k =
+  index_nat_to_intseq_le #U8 #SEC 32 (nat_from_intseq_le sc) k;
+  //assert (Seq.index (nat_to_intseq_le #U8 #SEC 32 (nat_from_intseq_le sc)) k ==
+  //        uint #U8 #SEC (nat_from_intseq_le sc / pow2 (8 * k) % pow2 8));
+  //assert (
+  //  nat_from_intseq_le sc ==
+  //  nat_from_intseq_le (nat_to_intseq_le #U8 #SEC 32 (nat_from_intseq_le sc)));
+  nat_from_intseq_le_inj sc (nat_to_intseq_le 32 (nat_from_intseq_le sc))
 
-    assert(nat_from_intseq_le (slice sc 0 k) < pow2 (k * 8));
-    small_div (nat_from_intseq_le (slice sc 0 k)) (pow2 (k * 8));
-    modulo_addition_lemma (uint_v sc.[k]) (pow2 8) (nat_from_bytes_le (slice sc (k + 1) 32));
-    lemma_u8_less sc.[k];
-    FStar.Math.Lemmas.small_mod (uint_v sc.[k]) (pow2 8)
 
-#reset-options "--z3refresh --z3rlimit 300"
+val lemma_euclidian_for_ithbit: k: nat -> i: nat
+  -> Lemma (k / (pow2 (8 * (i / 8)) * pow2 (i % 8)) == k / pow2 i)
 
-val lemma_euclidian_for_ithbit: k: nat ->i: nat -> Lemma (k / (pow2 (8 * (i/8)) * pow2 ( i % 8)) == k / (pow2 i))
-
-let lemma_euclidian_for_ithbit k i = 
+let lemma_euclidian_for_ithbit k i =
   lemma_div_def i 8;
-  pow2_plus (8 * (i/8)) (i % 8)
+  pow2_plus (8 * (i / 8)) (i % 8)
 
-val ith_bit: k: lbytes 32 -> i: nat {i < 256} -> Tot (t: uint64 {(uint_v t == 0 \/ uint_v t == 1) /\ uint_v t == (nat_from_intseq_le k) / pow2 i % 2})
 
-let ith_bit k i = 
-  let q = i / 8 in let r = i % 8 in
-  let tmp1 = k.[q] >>. (size r) in 
-  let tmp2 = tmp1 &. u8 1 in 
-  let res = to_u64 tmp2 in 
+val ith_bit: k:lbytes 32 -> i:nat{i < 256}
+  -> t:uint64 {(v t == 0 \/ v t == 1) /\ v t == nat_from_intseq_le k / pow2 i % 2}
+
+let ith_bit k i =
+  let q = i / 8 in
+  let r = i % 8 in
+  let tmp1 = k.[q] >>. (size r) in
+  let tmp2 = tmp1 &. u8 1 in
+  let res = to_u64 tmp2 in
   logand_le tmp1 (u8 1);
   logand_mask tmp1 (u8 1) 1;
   lemma_scalar_ith k q;
-  let k = nat_from_intseq_le k in 
-  pow2_modulo_division_lemma_1 (k / pow2 (8 * (i/8))) (i % 8) 8;
-  division_multiplication_lemma k (pow2 (8 * (i/8))) (pow2 (i % 8));
+  let k = nat_from_intseq_le k in
+  pow2_modulo_division_lemma_1 (k / pow2 (8 * (i / 8))) (i % 8) 8;
+  division_multiplication_lemma k (pow2 (8 * (i / 8))) (pow2 (i % 8));
   lemma_euclidian_for_ithbit k i;
   pow2_modulo_modulo_lemma_1 (k / pow2 i) 1 (8 - (i % 8));
   res
@@ -160,230 +138,275 @@ let ith_bit k i =
 let ( *% ) a b = (a * b) % prime
 
 
-val _exp_step0: p: nat_prime -> q: nat_prime -> Tot (t: tuple2 nat_prime nat_prime)
+val _exp_step0: p:nat_prime -> q:nat_prime -> tuple2 nat_prime nat_prime
 
-let _exp_step0 r0 r1 = 
-  let r1 = r0 *% r1 in 
-  let r0 = r0 *% r0 in 
+let _exp_step0 r0 r1 =
+  let r1 = r0 *% r1 in
+  let r0 = r0 *% r0 in
   r0, r1
 
-val _exp_step1: p: nat_prime -> q: nat_prime -> Tot (t: tuple2 nat_prime nat_prime)
 
-let _exp_step1 r0 r1 = 
-  let r0 = r0 *% r1 in 
-  let r1 = r1 *% r1 in 
+val _exp_step1: p:nat_prime -> q:nat_prime -> tuple2 nat_prime nat_prime
+
+let _exp_step1 r0 r1 =
+  let r0 = r0 *% r1 in
+  let r1 = r1 *% r1 in
   (r0, r1)
 
 
-val swap: p: nat_prime -> q: nat_prime -> Tot (r: tuple2 nat_prime nat_prime{let pNew, qNew = r in 
-  pNew == q /\ qNew == p})
-
-let swap p q = (q, p)
+let swap p q = q, p
 
 
-val conditional_swap: i: uint64 -> p: nat_prime -> q: nat_prime -> Tot (r: tuple2 nat_prime nat_prime
-  {
-    let pNew, qNew = r in 
-    if uint_v i = 0 then pNew == p /\ qNew == q
-    else
-      let p1, q1 = swap p q in 
-      p1 == pNew /\ q1 == qNew
- }
-)
+val conditional_swap: i:uint64 -> p:nat_prime -> q:nat_prime -> tuple2 nat_prime nat_prime
+
+let conditional_swap i p q =
+  if v i = 0 then (p, q) else (q, p)
 
 
-#reset-options "--z3refresh --z3rlimit  100"
-
-let conditional_swap i p q = 
-  if uint_v i = 0 then 
-    (p, q)
-  else
-    (q, p)
-
-val lemma_swaped_steps: p: nat_prime -> q: nat_prime -> 
+val lemma_swaped_steps: p: nat_prime -> q: nat_prime ->
   Lemma (
-    let (afterSwapP, afterSwapQ) = swap p q in 
-    let p1, q1 = _exp_step0 afterSwapP afterSwapQ in 
-    let p2, q2 = swap p1 q1 in 
-    let r0, r1 = _exp_step1 p q in 
+    let afterSwapP, afterSwapQ = swap p q in
+    let p1, q1 = _exp_step0 afterSwapP afterSwapQ in
+    let p2, q2 = swap p1 q1 in
+    let r0, r1 = _exp_step1 p q in
     p2 == r0 /\ q2 == r1)
 
 let lemma_swaped_steps p q = ()
 
-val _exp_step: k:  lseq uint8 32 ->  i: nat{i < 256} -> before: tuple2 nat_prime nat_prime -> Tot (t: tuple2 nat_prime nat_prime)
-    
-let _exp_step k i (p, q) = 
-  let bit = 255 - i in 
+
+val _exp_step: k:lseq uint8 32 -> i:nat{i < 256} -> before:tuple2 nat_prime nat_prime
+  -> tuple2 nat_prime nat_prime
+
+let _exp_step k i (p, q) =
+  let bit = 255 - i in
   let bit = ith_bit k bit in
   let open Lib.RawIntTypes in
-  if uint_to_nat bit = 0 then 
-      _exp_step0 p q 
-  else _exp_step1 p q  
+  if uint_to_nat bit = 0 then _exp_step0 p q else _exp_step1 p q
 
 
-#reset-options "--z3refresh --z3rlimit 300"
+val _exponent_spec: k:lseq uint8 32  -> tuple2 nat_prime nat_prime
+  -> tuple2 nat_prime nat_prime
 
-val _exponent_spec: k: lseq uint8 32  -> tuple2 nat_prime nat_prime -> Tot (tuple2 nat_prime nat_prime)
-
-let _exponent_spec k (p, q) = 
-  let open Lib.LoopCombinators in 
+let _exponent_spec k (p, q) =
+  let open Lib.LoopCombinators in
   Lib.LoopCombinators.repeati 256 (_exp_step k) (p, q)
 
 
-val lemma_even: index : nat {index <= 256 && index > 0} -> k: lseq uint8 32 {uint_v (ith_bit k (256 - index)) == 0} -> 
+val lemma_even: index:pos{index <= 256} -> k:lseq uint8 32 {v (ith_bit k (256 - index)) == 0} ->
   Lemma (
-    let number = nat_from_bytes_le k in 
-    let newIndex = 256 - index in 
-    2 * arithmetic_shift_right number (newIndex + 1) == arithmetic_shift_right number newIndex)
+    let number = nat_from_bytes_le k in
+    let newIndex = 256 - index in
+    2 * arithmetic_shift_right number (newIndex + 1) ==
+    arithmetic_shift_right number newIndex)
 
-let lemma_even index k = 
-  let number = nat_from_bytes_le k in 
-  let n = 256 - index in 
+let lemma_even index k =
+  let number = nat_from_bytes_le k in
+  let n = 256 - index in
   FStar.Math.Lemmas.pow2_double_mult n;
-  lemma_div_def (number / (pow2 n)) 2;
+  lemma_div_def (number / pow2 n) 2;
   FStar.Math.Lemmas.division_multiplication_lemma number (pow2 n) 2
 
-val lemma_odd: index: nat{index <= 256 && index > 0} -> k: lseq uint8 32 {uint_v (ith_bit k (256 - index)) == 1} -> 
-  Lemma(
-    let number = nat_from_intseq_le k in 
-    let n = 256 - index  in 
-    2 * arithmetic_shift_right number (n + 1) + 1 == arithmetic_shift_right number n)
 
-let lemma_odd index k = 
-  let number = nat_from_bytes_le k in 
-  let n = 256 - index in 
-  let a0 = 2 * arithmetic_shift_right number (n + 1) + 1 in 
-  lemma_div_def (number / (pow2 n)) 2;
+val lemma_odd: index:pos{index <= 256} -> k:lseq uint8 32 {uint_v (ith_bit k (256 - index)) == 1} ->
+  Lemma(
+    let number = nat_from_intseq_le k in
+    let n = 256 - index  in
+    2 * arithmetic_shift_right number (n + 1) + 1 ==
+    arithmetic_shift_right number n)
+
+let lemma_odd index k =
+  let number = nat_from_bytes_le k in
+  let n = 256 - index in
+  let a0 = 2 * arithmetic_shift_right number (n + 1) + 1 in
+  lemma_div_def (number / pow2 n) 2;
   division_multiplication_lemma number (pow2 n) 2;
   pow2_double_mult n;
-  assert(arithmetic_shift_right number (n + 1) == number / (pow2 (n + 1)));
-  assert(arithmetic_shift_right number n == 2 * arithmetic_shift_right number (n + 1) + 1)
+  assert (arithmetic_shift_right number (n + 1) == number / pow2 (n + 1));
+  assert (arithmetic_shift_right number n ==
+          2 * arithmetic_shift_right number (n + 1) + 1)
 
 
-val lemma_exponen_spec: k: lseq uint8 32 -> start: tuple2 nat_prime nat_prime {let st0, st1 = start in st0 == 1}  -> 
-  index: nat {index <= 256} ->
+val lemma_exponen_spec: k:lseq uint8 32
+  -> start:tuple2 nat_prime nat_prime {let st0, st1 = start in st0 == 1}
+  -> index:nat{index <= 256} ->
   Lemma (
-    let start0, start1 = start in 
-    let number = nat_from_bytes_le k in 
-    let newIndex = 256 - index in 
-    let f0, f1 = Lib.LoopCombinators.repeati index (_exp_step k) start in 
-    f0 == pow start1 (FStar.Math.Lib.arithmetic_shift_right number newIndex) % prime_p256_order /\
-    f1 == pow start1 ((FStar.Math.Lib.arithmetic_shift_right number newIndex) + 1) % prime_p256_order
-    )
+    let start0, start1 = start in
+    let number = nat_from_bytes_le k in
+    let newIndex = 256 - index in
+    let f0, f1 = Lib.LoopCombinators.repeati index (_exp_step k) start in
+    f0 == pow start1 (arithmetic_shift_right number newIndex) % prime_p256_order /\
+    f1 == pow start1 (arithmetic_shift_right number newIndex + 1) % prime_p256_order
+  )
 
-let rec lemma_exponen_spec k start index = 
-  let open FStar.Math.Lib in 
-  let open FStar.Math.Lemmas in 
-  let open Lib.RawIntTypes in 
-  let f = _exp_step k in 
-  let st0, st1 = start in 
-  let number = nat_from_bytes_le k in 
-  let newIndex = 256 - index in 
-let open Lib.LoopCombinators in 
+#push-options "--fuel 2 --z3rlimit 300"
+
+let rec lemma_exponen_spec k start index =
+  let open FStar.Math.Lib in
+  let open FStar.Math.Lemmas in
+  let open Lib.RawIntTypes in
+  let f = _exp_step k in
+  let st0, st1 = start in
+  let number = nat_from_bytes_le k in
+  let newIndex = 256 - index in
+  let open Lib.LoopCombinators in
   match index with
-  | 0 ->  eq_repeati0 256 (_exp_step k) start;
+  | 0 -> eq_repeati0 256 (_exp_step k) start;
     assert_norm (FStar.Math.Lib.arithmetic_shift_right number newIndex == 0)
-  | _ -> begin
+  | _ ->
+    begin
     unfold_repeati 256 f start (index - 1);
     lemma_exponen_spec k start (index - 1);
-    let bitMask = uint_v (ith_bit k (256 - index)) in 
-    match bitMask with 
-      | 0 -> 
-	let a0 = pow st1 (arithmetic_shift_right number (256 - index + 1)) in 
-	let a1 = pow st1 (arithmetic_shift_right number (256 - index + 1) + 1) in 
-	
-	modulo_distributivity_mult a0 a0 prime_p256_order;	
-	modulo_distributivity_mult a0 a1 prime_p256_order;
-	
-	pow_plus st1 (arithmetic_shift_right number (256 - index + 1)) (arithmetic_shift_right number (256 - index + 1));
-	pow_plus st1 (arithmetic_shift_right number (256 - index + 1)) (arithmetic_shift_right number (256 - index + 1) + 1); 
-	
-	lemma_even index k
-      | 1 -> 
-	let a0 = pow st1 (arithmetic_shift_right number (256 - index + 1)) in 
-	let a1 = pow st1 (arithmetic_shift_right number (256 - index + 1) + 1) in 
+    let bitMask = uint_v (ith_bit k (256 - index)) in
+    match bitMask with
+      | 0 ->
+        let a0 = pow st1 (arithmetic_shift_right number (256 - index + 1)) in
+        let a1 = pow st1 (arithmetic_shift_right number (256 - index + 1) + 1) in
 
-	modulo_distributivity_mult a0 a1 prime_p256_order;
-	modulo_distributivity_mult a1 a1 prime_p256_order;
-	pow_plus st1 (arithmetic_shift_right number (256 - index + 1)) (arithmetic_shift_right number (256 - index + 1) + 1);
-	pow_plus st1 (arithmetic_shift_right number (256 - index + 1) + 1) (arithmetic_shift_right number (256 - index + 1) + 1);
+        modulo_distributivity_mult a0 a0 prime_p256_order;
+        modulo_distributivity_mult a0 a1 prime_p256_order;
 
-	lemma_odd index k
+        pow_plus st1 (arithmetic_shift_right number (256 - index + 1)) (arithmetic_shift_right number (256 - index + 1));
+        pow_plus st1 (arithmetic_shift_right number (256 - index + 1)) (arithmetic_shift_right number (256 - index + 1) + 1);
+
+        lemma_even index k
+      | 1 ->
+        let a0 = pow st1 (arithmetic_shift_right number (256 - index + 1)) in
+        let a1 = pow st1 (arithmetic_shift_right number (256 - index + 1) + 1) in
+
+        modulo_distributivity_mult a0 a1 prime_p256_order;
+        modulo_distributivity_mult a1 a1 prime_p256_order;
+        pow_plus st1 (arithmetic_shift_right number (256 - index + 1)) (arithmetic_shift_right number (256 - index + 1) + 1);
+        pow_plus st1 (arithmetic_shift_right number (256 - index + 1) + 1) (arithmetic_shift_right number (256 - index + 1) + 1);
+
+        lemma_odd index k
     end
 
+#pop-options
 
-unfold let prime_p256_order_inverse_list: list uint8 = 
-   [
-     (u8 79); (u8 37); (u8 99); (u8 252); (u8 194); (u8 202); (u8 185); (u8 243); 
-     (u8 132); (u8 158); (u8 23); (u8 167); (u8 173); (u8 250); (u8 230); (u8 188); 
-     (u8 255); (u8 255); (u8 255); (u8 255); (u8 255); (u8 255); (u8 255); (u8 255);
-     (u8 0); (u8 0); (u8 0); (u8 0); (u8 255); (u8 255); (u8 255); (u8 255)
-   ]
+#push-options "--ifuel 1"
 
-let prime_p256_order_inverse_seq: lseq uint8 32 = 
+val nat_from_intlist_le: #t:inttype{unsigned t} -> #l:secrecy_level
+  -> b:list (uint_t t l) -> nat
+
+let rec nat_from_intlist_le #t #l = function
+  | [] -> 0
+  | hd :: tl -> v hd + pow2 (bits t) * nat_from_intlist_le tl
+
+#pop-options
+
+#push-options "--fuel 1"
+
+val index_seq_of_list_cons: #a:Type -> x:a -> l:list a -> i:nat{i < List.Tot.length l} -> Lemma
+  (Seq.index (Seq.seq_of_list (x::l)) (i+1) == Seq.index (Seq.seq_of_list l) i)
+
+let index_seq_of_list_cons #a x l i =
+  assert (Seq.index (Seq.seq_of_list (x::l)) (i+1) == List.Tot.index (x::l) (i+1))
+
+
+val nat_from_intlist_seq_le: #t:inttype{unsigned t} -> #l:secrecy_level
+  -> len:size_nat -> b:list (uint_t t l){List.Tot.length b = len}
+  -> Lemma (nat_from_intlist_le b == nat_from_intseq_le (of_list b))
+
+let rec nat_from_intlist_seq_le #t #l len b =
+  match b with
+  | [] -> ()
+  | hd :: tl ->
+    begin
+    let s = of_list b in
+    Classical.forall_intro (index_seq_of_list_cons hd tl);
+    assert (equal (of_list tl) (slice s 1 len));
+    assert (index s 0 == List.Tot.index b 0);
+    nat_from_intseq_le_lemma0 (slice s 0 1);
+    nat_from_intseq_le_slice_lemma s 1;
+    nat_from_intlist_seq_le (len - 1) tl
+    end
+
+#pop-options
+
+unfold let prime_p256_order_inverse_list: list uint8 =
+ [
+   u8 79;  u8 37;  u8 99;  u8 252; u8 194; u8 202; u8 185; u8 243;
+   u8 132; u8 158; u8 23;  u8 167; u8 173; u8 250; u8 230; u8 188;
+   u8 255; u8 255; u8 255; u8 255; u8 255; u8 255; u8 255; u8 255;
+   u8 0;   u8 0;   u8 0;   u8 0;   u8 255; u8 255; u8 255; u8 255
+ ]
+
+
+let prime_p256_order_inverse_seq: s:lseq uint8 32{nat_from_intseq_le s == prime_p256_order - 2} =
   assert_norm (List.Tot.length prime_p256_order_inverse_list == 32);
+  nat_from_intlist_seq_le 32 prime_p256_order_inverse_list;
+  assert_norm (nat_from_intlist_le prime_p256_order_inverse_list == prime_p256_order - 2);
   of_list prime_p256_order_inverse_list
 
 
-unfold let prime_p256_order_list: list uint8 = 
-   [
-     (u8 81); (u8 37); (u8 99); (u8 252); (u8 194); (u8 202); (u8 185); (u8 243); 
-     (u8 132); (u8 158); (u8 23); (u8 167); (u8 173); (u8 250); (u8 230); (u8 188); 
-     (u8 255); (u8 255); (u8 255); (u8 255); (u8 255); (u8 255); (u8 255); (u8 255);
-     (u8 0); (u8 0); (u8 0); (u8 0); (u8 255); (u8 255); (u8 255); (u8 255)
-   ]
+unfold let prime_p256_order_list: list uint8 =
+ [
+   u8 81;  u8 37;  u8 99;  u8 252; u8 194; u8 202; u8 185; u8 243;
+   u8 132; u8 158; u8 23;  u8 167; u8 173; u8 250; u8 230; u8 188;
+   u8 255; u8 255; u8 255; u8 255; u8 255; u8 255; u8 255; u8 255;
+   u8 0;   u8 0;   u8 0;   u8 0;   u8 255; u8 255; u8 255; u8 255
+ ]
 
-let prime_p256_order_seq: lseq uint8 32 = 
+
+let prime_p256_order_seq: s:lseq uint8 32{nat_from_intseq_le s == prime_p256_order} =
   assert_norm (List.Tot.length prime_p256_order_list == 32);
+  nat_from_intlist_seq_le 32 prime_p256_order_list;
+  assert_norm (nat_from_intlist_le prime_p256_order_list == prime_p256_order);
   of_list prime_p256_order_list
 
 open Hacl.Spec.P256.Definitions
 
+val exponent_spec: a:nat_prime -> r:nat_prime{r = pow a (prime_p256_order - 2) % prime_p256_order}
 
-#reset-options "--z3refresh --z3rlimit  100"
-val exponent_spec: a: nat_prime -> Tot (r: nat_prime {r = pow a (prime_p256_order - 2) % prime_p256_order})
-
-let exponent_spec a = 
-  let a0, _ = _exponent_spec prime_p256_order_inverse_seq (1, a) in 
+let exponent_spec a =
+  let a0, _ = _exponent_spec prime_p256_order_inverse_seq (1, a) in
   lemma_exponen_spec prime_p256_order_inverse_seq (1, a) 256;
-  assume (nat_from_intseq_le prime_p256_order_inverse_seq = prime_p256_order - 2);
   a0
 
 
-val changeEndian: i: felem_seq -> Tot felem_seq
+val changeEndian: felem_seq -> felem_seq
 
-let changeEndian i = 
-  let zero =  Lib.Sequence.index i 0 in 
-  let one =   Lib.Sequence.index i 1 in 
-  let two =   Lib.Sequence.index i 2 in 
-  let three = Lib.Sequence.index i 3 in 
+let changeEndian i =
+  let zero =  Lib.Sequence.index i 0 in
+  let one =   Lib.Sequence.index i 1 in
+  let two =   Lib.Sequence.index i 2 in
+  let three = Lib.Sequence.index i 3 in
 
-  let o = Lib.Sequence.upd i 0 three in 
-  let o = Lib.Sequence.upd o 1 two in 
-  let o = Lib.Sequence.upd o 2 one in 
-	  Lib.Sequence.upd o 3 zero
+  let o = Lib.Sequence.upd i 0 three in
+  let o = Lib.Sequence.upd o 1 two in
+  let o = Lib.Sequence.upd o 2 one in
+          Lib.Sequence.upd o 3 zero
 
 
-val verifyQValidCurvePointSpec: 
+val verifyQValidCurvePointSpec:
   publicKey:tuple3 nat nat nat{~(isPointAtInfinity publicKey)} -> bool
 
-let verifyQValidCurvePointSpec publicKey = 
-  let x, y, z = publicKey in 
-  x < prime256 && 
-  y < prime256 && 
-  z < prime256 && 
+let verifyQValidCurvePointSpec publicKey =
+  let x, y, z = publicKey in
+  x < prime256 &&
+  y < prime256 &&
+  z < prime256 &&
   isPointOnCurve (x, y, z) &&
   isPointAtInfinity (scalar_multiplication prime_p256_order_seq publicKey)
 
 
-val checkCoordinates: r: nat -> s: nat -> bool
+val checkCoordinates: r:nat -> s:nat -> bool
 
 let checkCoordinates r s =
-  if r > 0 && r < prime_p256_order && s > 0 && s < prime_p256_order then true else false
+  if r > 0 && r < prime_p256_order && s > 0 && s < prime_p256_order
+  then true
+  else false
+
+
+unfold
+let basePoint: point_nat =
+  (0x6B17D1F2E12C4247F8BCE6E563A440F277037D812DEB33A0F4A13945D898C296,
+   0x4FE342E2FE1A7F9B8EE7EB4A7C0F9E162BCE33576B315ECECBB6406837BF51F5,
+   1)
 
 
 val ecdsa_verification: publicKey:tuple2 nat nat -> r:nat -> s:nat
-  -> mLen:size_nat{mLen < Spec.Hash.Definitions.(max_input_length SHA2_256)}
+  -> mLen:size_nat{mLen < Def.(max_input_length SHA2_256)}
   -> input:lseq uint8 mLen
   -> bool
 
@@ -396,12 +419,10 @@ let ecdsa_verification publicKey r s mLen input =
     else
       begin
       let open Lib.ByteSequence in
-      let hashResult = H.hash Def.SHA2_256 input in
+      let hashResult = Spec.Agile.Hash.hash Def.SHA2_256 input in
       let hashNat = nat_from_intseq_le (changeEndian(uints_from_bytes_be hashResult)) % prime_p256_order in
       let u1 = nat_to_bytes_le 32 (pow s (prime_p256_order - 2) * hashNat % prime_p256_order) in
       let u2 = nat_to_bytes_le 32 (pow s (prime_p256_order - 2) * r % prime_p256_order) in
-
-      let basePoint = (0x6B17D1F2E12C4247F8BCE6E563A440F277037D812DEB33A0F4A13945D898C296, 0x4FE342E2FE1A7F9B8EE7EB4A7C0F9E162BCE33576B315ECECBB6406837BF51F5, 1) in
       let pointAtInfinity = (0, 0, 0) in
       let u1D, _ = montgomery_ladder_spec u1 (pointAtInfinity, basePoint) in
       let u2D, _ = montgomery_ladder_spec u2 (pointAtInfinity, publicJacobian) in
@@ -413,48 +434,46 @@ let ecdsa_verification publicKey r s mLen input =
   end
 
 
-val ecdsa_signature_nist_compliant: 
-  input: lseq uint8 32 -> 
-  privateKey: lseq uint8 32 -> 
-  k: lseq uint8 32 -> 
-  Tot (tuple3 nat nat uint64)
+val ecdsa_signature_nist_compliant:
+    input:lseq uint8 32
+  -> privateKey:lseq uint8 32
+  -> k:lseq uint8 32
+  -> tuple3 nat nat uint64
 
-let ecdsa_signature_nist_compliant  input privateKey k = 
-  let basePoint = (0x6B17D1F2E12C4247F8BCE6E563A440F277037D812DEB33A0F4A13945D898C296, 0x4FE342E2FE1A7F9B8EE7EB4A7C0F9E162BCE33576B315ECECBB6406837BF51F5, 1) in
-  let (rxN, ryN, rzN), _ = montgomery_ladder_spec k ((0,0,0), basePoint) in 
-  let (xN, _, _) = _norm (rxN, ryN, rzN) in 
-  let z = nat_from_bytes_le input in 
-  let kFelem = nat_from_bytes_le k in 
-  let privateKey = nat_from_bytes_le privateKey in 
+let ecdsa_signature_nist_compliant input privateKey k =
+  let (rxN, ryN, rzN), _ = montgomery_ladder_spec k ((0,0,0), basePoint) in
+  let (xN, _, _) = _norm (rxN, ryN, rzN) in
+  let z = nat_from_bytes_le input in
+  let kFelem = nat_from_bytes_le k in
+  let privateKey = nat_from_bytes_le privateKey in
   let resultR = xN % prime_p256_order in
-  let resultS = (z + resultR * privateKey) * pow kFelem (prime_p256_order - 2) % prime_p256_order in 
-    if resultR = 0 || resultS = 0 then 
+  let resultS = (z + resultR * privateKey) * pow kFelem (prime_p256_order - 2) % prime_p256_order in
+    if resultR = 0 || resultS = 0 then
       resultR, resultS, u64 (pow2 64 - 1)
-    else 
+    else
       resultR, resultS, u64 0
 
 
-val ecdsa_signature: 
-  mLen: size_nat{mLen < Spec.Hash.Definitions.max_input_length Spec.Hash.Definitions.SHA2_256} -> 
-  input: lseq uint8 mLen -> 
-  privateKey: lseq uint8 32 -> 
-  k: lseq uint8 32 -> 
-  Tot (tuple3 nat nat uint64)
+val ecdsa_signature:
+    mLen:size_nat{mLen < Def.(max_input_length SHA2_256)}
+  -> input:lseq uint8 mLen
+  -> privateKey:lseq uint8 32
+  -> k:lseq uint8 32
+  -> tuple3 nat nat uint64
 
-let ecdsa_signature mLen input privateKey k = 
-  let basePoint = (0x6B17D1F2E12C4247F8BCE6E563A440F277037D812DEB33A0F4A13945D898C296, 0x4FE342E2FE1A7F9B8EE7EB4A7C0F9E162BCE33576B315ECECBB6406837BF51F5, 1) in
-  let (rxN, ryN, rzN), _ = montgomery_ladder_spec k ((0,0,0), basePoint) in 
-  let (xN, _, _) = _norm (rxN, ryN, rzN) in 
-  
-  let hashM = H.hash Def.SHA2_256 input in 
+let ecdsa_signature mLen input privateKey k =
+  let (rxN, ryN, rzN), _ = montgomery_ladder_spec k ((0,0,0), basePoint) in
+  let (xN, _, _) = _norm (rxN, ryN, rzN) in
+
+  let hashM = Spec.Agile.Hash.hash Def.SHA2_256 input in
   let hashChanged = changeEndian (uints_from_bytes_be hashM) in
-  let z = nat_from_intseq_le hashChanged % prime_p256_order in 
-  
-  let kFelem = nat_from_bytes_le k in 
-  let privateKey = nat_from_bytes_le privateKey in 
+  let z = nat_from_intseq_le hashChanged % prime_p256_order in
+
+  let kFelem = nat_from_bytes_le k in
+  let privateKey = nat_from_bytes_le privateKey in
   let resultR = xN % prime_p256_order in
-  let resultS = (z + resultR * privateKey) * pow kFelem (prime_p256_order - 2) % prime_p256_order in 
-    if resultR = 0 || resultS = 0 then 
+  let resultS = (z + resultR * privateKey) * pow kFelem (prime_p256_order - 2) % prime_p256_order in
+    if resultR = 0 || resultS = 0 then
       resultR, resultS, u64 (pow2 64 - 1)
-    else 
+    else
       resultR, resultS, u64 0
